process/subject_reduction.v
@@ -1,4 +1,4 @@
-From SST Require Export src.expressions process.processes process.typecheck type.global type.local process.beta process.sessions process.inversion  type.isomorphism type.projection.
+From SST Require Export src.expressions process.processes process.typecheck type.global type.local process.beta process.sessions process.inversion  type.isomorphism type.projection type.proj_sub.
 Require Import List String Datatypes ZArith Relations PeanoNat.
 Open Scope list_scope.
 From Paco Require Import paco pacotac.
@@ -12,77 +12,6 @@ Inductive multiC : relation gtt :=
   
 
 
-
-(* Lemma proj_all : 
-       wfgC G -> 
-       projectionC G p T ->
-       wfC T.
- *)
-Lemma projection_wfc_p : forall G l p q x4 x8 x9, 
-        wfgC G ->
-        wfC (ltt_recv q x4) ->
-        projectionC G p (ltt_recv q x4) ->
-        gttstepC G x8 q p l ->
-        projectionC x8 p x9 ->
-        wfC x9.
-Admitted.
-
-Lemma projection_wfc_q : forall G l p q x x8 x9,
-        wfgC G ->
-        wfC (ltt_send p x) ->
-        projectionC G q (ltt_send p x) ->
-        gttstepC G x8 q p l ->
-        projectionC x8 q x9 ->
-        wfC x9.
-Admitted.
-
-Lemma projection_wfc_r : forall G l p0 q s x x0 x6,
-        wfgC G ->
-        wfC x ->
-        q <> s ->
-        p0 <> s ->
-        projectionC G s x ->
-        gttstepC G x6 q p0 l ->
-        projectionC x6 s x0 ->
-        wfC x0.
-Admitted.
-
-Lemma _3_19_h : forall p q l G L1 L2 S T xs y,
-  wfgC G ->
-  projectionC G p (ltt_send q L1) -> 
-  subtypeC (ltt_send q (extendLis l (Datatypes.Some(S,T)))) (ltt_send q L1) ->
-  projectionC G q (ltt_recv p L2) -> 
-  onth l xs = Some y ->
-  subtypeC (ltt_recv p xs) (ltt_recv p L2) -> 
-  exists G', gttstepC G G' p q l.
-Proof.
-  intros. 
-  pinversion H0. subst.
-  pinversion H1; subst; try easy.
-  - admit.
-  - admit.
-Admitted.
-
-Lemma _3_19_2 : forall p q l G G' L1 L2 S T xs,
-  wfgC G ->
-  projectionC G q (ltt_recv p L1) -> 
-  subtypeC (ltt_recv p xs) (ltt_recv p L1) ->
-  onth l xs = Some (S, T) ->
-  gttstepC G G' p q l -> 
-  projectionC G' q L2 ->
-  subtypeC T L2.
-Admitted.
-
-Lemma _3_19_3 : forall p q r l G G' L1 L2,
-  wfgC G ->
-  r <> p -> r <> q ->
-  projectionC G r L1 ->
-  gttstepC G G' p q l -> 
-  projectionC G' r L2 -> 
-  subtypeC L1 L2.
-Proof.
-  
-Admitted.
 
 Lemma _3_21_1_helper : forall l x1 xs x4 x5 y,
     onth l x1 = Some (x4, x5) ->
@@ -117,52 +46,52 @@ Proof.
   split; try easy. apply Classical_Prop.and_not_or. split; try easy.
 Qed.
 
-Lemma _3_21_3_helper : forall M p q x6 G l,
+
+
+Lemma _3_21_3_helper : forall M p q G G' l L1 L2 S T xs y,
     wfgC G ->
+    projectionC G p (ltt_send q L1) -> 
+    subtypeC (ltt_send q (extendLis l (Datatypes.Some(S, T)))) (ltt_send q L1) ->
+    projectionC G q (ltt_recv p L2) -> 
+    onth l xs = Some y ->
     ForallT
        (fun (u : string) (P : process) =>
         exists T : ltt, projectionC G u T /\ typ_proc nil nil P T) M ->
-    gttstepC G x6 q p l ->
+    subtypeC (ltt_recv p xs) (ltt_recv p L2) -> 
+    gttstepC G G' p q l ->
     ~ InT q M ->
     ~ InT p M ->
     ForallT
       (fun (u : string) (P : process) =>
-       exists T : ltt, projectionC x6 u T /\ typ_proc nil nil P T) M.
+       exists T : ltt, projectionC G' u T /\ typ_proc nil nil P T) M.
 Proof.
   intro M. induction M; intros; try easy.
-  - constructor; try easy. 
-    inversion H0. subst. destruct H5. destruct H4.
-    specialize(projection_cont_r G x6 q p0 l s x H H4 H1); intros.
-    assert (q <> s). { 
-      unfold InT in H1. simpl in H1. 
-      specialize(Classical_Prop.not_or_and (s = q) False H2); intros. destruct H7.
-      easy.
-    }
-    assert (p0 <> s). {
-      unfold InT in H3. simpl in H3.
-      specialize(Classical_Prop.not_or_and (s = p0) False H3); intros. destruct H8.
-      easy.
-    }
-    specialize(H6 H7 H8). destruct H6.
-    exists x0.
-    split; try easy.
-    apply tc_sub with (t := x); try easy.
-    specialize(_3_19_3 q p0 s l G x6 x x0); intros.
-    apply H9; try easy.
-    assert (wfC x0). { 
-        specialize(projection_wfc_r G l p0 q s x x0 x6); intros.
-        apply H9; try easy.
-        specialize(typable_implies_wfC H5). easy.
-    } easy. 
-  - inversion H0. subst. simpl in *.
-    unfold InT in *. simpl in *.
-    specialize(noin_cat_and q (flattenT M1) (flattenT M2) H2); intros.
-    specialize(noin_cat_and p (flattenT M1) (flattenT M2) H3); intros.
-    specialize(Classical_Prop.not_or_and (InT q M1) (InT q M2) H4); intros. destruct H8. 
-    specialize(Classical_Prop.not_or_and (InT p M1) (InT p M2) H5); intros. destruct H10.
-    constructor. apply IHM1 with (p := p) (q := q) (G := G) (l := l); try easy.
-    apply IHM2 with (p := p) (q := q) (G := G) (l := l); try easy.
-Qed.
+  - unfold InT in *. simpl in H7. simpl in H8.
+    specialize(Classical_Prop.not_or_and (s = q) False H7); intros. destruct H9.
+    specialize(Classical_Prop.not_or_and (s = p0) False H8); intros. destruct H11.
+    clear H10 H12 H7 H8.
+    constructor.
+    inversion H4. subst. destruct H8 as [T' H8]. destruct H8.
+    assert(exists T, projectionC G' s T /\ subtypeC T' T).
+    {
+      admit.
+    } 
+    destruct H10. destruct H10.
+    exists x. split; try easy. apply tc_sub with (t := T'); try easy.
+    admit. (* wfC *)
+  - inversion H4. subst.
+    specialize(noin_cat_and q (flattenT M1) (flattenT M2) H7); intros.
+    specialize(noin_cat_and p (flattenT M1) (flattenT M2) H8); intros.
+    specialize(Classical_Prop.not_or_and (In q (flattenT M1)) (In q (flattenT M2)) H9); intros.
+    specialize(Classical_Prop.not_or_and (In p (flattenT M1)) (In p (flattenT M2)) H10); intros.
+    destruct H13. destruct H14.
+    unfold InT in *.
+    specialize(IHM1 p q G G' l L1 L2 S T xs y H H0 H1 H2 H3 H11 H5 H6 H13 H14).
+    specialize(IHM2 p q G G' l L1 L2 S T xs y H H0 H1 H2 H3 H12 H5 H6 H15 H16).
+    constructor; try easy.
+Admitted.
+
+
 
 Lemma _3_21_helper : forall l xs x1 y,
     onth l xs = Some y ->
@@ -232,39 +161,37 @@ Proof.
       constructor; try easy.
     constructor. constructor. 
     - constructor.
-      specialize(_3_19_2 q p l G G' x4); intros.
-      specialize(projection_cont_p G G' p q l x4 H23 H30 H1); intros.
-      destruct H34. exists x10. split; try easy.
-      specialize(H33 x10 x0 x5 x1 H23 H1 H12 H21 H30 H34).
+      specialize(_3_19_2 q p l G G' x x4 x2 x3 x0 x5 x1 H23 H5 H17 H1 H21 H12 H30); intros.
+      destruct H33. destruct H33. exists x10. split; try easy.
       apply _a24 with (S := x0); try easy.
       - apply tc_sub with (t := x5); try easy.
         assert (wfC x10). 
         {
-          specialize(projection_wfc_p G l p q x4 G' x10); intros.
-          apply H35; try easy. 
-          specialize(typable_implies_wfC H3). easy.
+          admit.
+          (* apply H35; try easy. 
+          specialize(typable_implies_wfC H3). easy. *)
         }
         easy.
       - apply sc_sub with (s := x2); try easy.
         apply expr_typ_multi with (e := e); intros; try easy.
         apply sstrans with (s2 := x9); try easy.
     - constructor.
-      specialize(_3_19_1 q p l G G' x); intros.
-      specialize(projection_cont_q G G' p q l x H23 H30 H5); intros.
-      destruct H34. exists x10. split; try easy.
-      specialize(H33 x10 x2 x3 H23 H5 H17 H30 H34).
-      apply tc_sub with (t := x3); try easy.
-      assert (wfC x10).
-      {
-        specialize(projection_wfc_q G l p q x G' x10); intros.
-        apply H35; try easy.
-        specialize(typable_implies_wfC H10). easy.
-      }
-      easy.
-    - apply _3_21_3_helper with (p := p) (q := q) (G := G) (l := l); try easy.
-      inversion H7. subst. easy.
+      specialize(_3_19_1 q p l G G' x x4 x2 x3 x0 x5 x1 H23 H5 H17 H1 H21 H12 H30); intros.
+      destruct H33. destruct H33. exists x10. split; try easy.
+      - apply tc_sub with (t := x3); try easy.
+        assert (wfC x10).
+        {
+          admit.
+         (*  specialize(projection_wfc_q G l p q x G' x10); intros.
+          apply H35; try easy.
+          specialize(typable_implies_wfC H10). easy. *)
+        }
+        easy.
+    - specialize(_3_21_3_helper M q p G G' l x x4 x2 x3 x1 (x0, x5)); intros.
+      apply H33; try easy.
       simpl in H6. specialize(Classical_Prop.not_or_and (q = p) (In p (flattenT M)) H6); intros.
-      destruct H33; try easy. 
+      destruct H34; try easy. unfold InT. 
+      inversion H7. subst. easy.
 
   (* T-COND *)
   inversion H0. subst. rename H3 into H100. rename H4 into H101. rename H5 into H102. rename H6 into H103. rename H7 into H3. 
