type/isomorphism.v
@@ -89,3 +89,4 @@ Definition wfC T := exists T', lttTC T' T /\ wfL T' /\ (forall n, exists m, guar
 
 
 
+
