type/local.v
@@ -485,6 +485,422 @@ Qed.
 
 
 
+Lemma mon_lttT : monotone2 lttT.
+Proof.
+  unfold monotone2. intros. induction IN; intros; try easy.
+  - apply lttT_end.
+  - apply lttT_send; try easy.
+    - revert H LE. revert r r' p ys.
+      induction xs; intros; try easy.
+      destruct ys; try easy.
+      destruct ys; try easy.
+      inversion H. subst.
+      constructor.
+      - destruct H3. left. easy.
+        destruct H0. destruct H0. destruct H0. destruct H0. destruct H1. subst. right.
+        exists x. exists x0. exists x1. split; try easy. split; try easy.
+        apply LE; try easy.
+      - apply IHxs with (r := r); try easy.
+  - apply lttT_recv; try easy.
+    - revert H LE. revert r r' p ys.
+      induction xs; intros; try easy.
+      destruct ys; try easy.
+      destruct ys; try easy.
+      inversion H. subst.
+      constructor.
+      - destruct H3. left. easy.
+        destruct H0. destruct H0. destruct H0. destruct H0. destruct H1. subst. right.
+        exists x. exists x0. exists x1. split; try easy. split; try easy.
+        apply LE; try easy.
+      - apply IHxs with (r := r); try easy.
+  - apply lttT_rec with (Q := Q); try easy.
+
+Qed.
+
+Lemma triad_le :  forall m t',
+                  is_true (ssrnat.leq m t') ->
+                  is_true (ssrnat.leq (S t') m) -> False.
+Proof.
+Admitted.
+  
+
+Lemma subst_injL : forall m n G G1 Q Q0, subst_local m n G G1 Q0 -> subst_local m n G G1 Q -> Q = Q0.
+Proof.
+  intros m n G G1.
+  revert m n G. induction G1 using local_ind_ref; intros; try easy.
+  inversion H. subst. 
+  - inversion H0; try easy. 
+  - subst. inversion H0; try easy.
+  - subst. inversion H0; try easy.
+    subst. specialize(triad_le m t' H6 H8); try easy.
+  - subst. inversion H0; try easy. 
+    subst. specialize(triad_le m t' H8 H6); try easy.
+  
+  inversion H. subst. inversion H0. subst. easy.
+  
+  inversion H0. subst. inversion H1. subst.
+  assert (ys0 = ys). {
+    clear H0 H1. revert H H8 H9. revert p m n G ys ys0.
+    induction lis; intros; try easy.
+    destruct ys; try easy. destruct ys0; try easy.
+    destruct ys; try easy. destruct ys0; try easy.
+    inversion H. subst. clear H.
+    inversion H8. subst. clear H8.
+    inversion H9. subst. clear H9.
+    specialize(IHlis p m n G ys ys0 H3 H6 H8). subst.
+    clear H3 H6 H8.
+    destruct H4. destruct H. subst.
+    destruct H5. destruct H. subst. easy.
+    destruct H. destruct H. destruct H. easy.
+    destruct H. destruct H. destruct H. destruct H. destruct H0. subst.
+    destruct H5; try easy.
+    destruct H. destruct H. destruct H. destruct H. destruct H0. 
+    inversion H. subst. 
+    destruct H2; try easy. destruct H0. destruct H0. destruct H0. 
+    inversion H0. subst.
+    specialize(H2 m n G x1 x4 H3 H1). subst. easy.
+  }
+  subst. easy.
+  
+  inversion H0. subst. inversion H1. subst.
+  assert (ys0 = ys). {
+    clear H0 H1. revert H H8 H9. revert p m n G ys ys0.
+    induction lis; intros; try easy.
+    destruct ys; try easy. destruct ys0; try easy.
+    destruct ys; try easy. destruct ys0; try easy.
+    inversion H. subst. clear H.
+    inversion H8. subst. clear H8.
+    inversion H9. subst. clear H9.
+    specialize(IHlis p m n G ys ys0 H3 H6 H8). subst.
+    clear H3 H6 H8.
+    destruct H4. destruct H. subst.
+    destruct H5. destruct H. subst. easy.
+    destruct H. destruct H. destruct H. easy.
+    destruct H. destruct H. destruct H. destruct H. destruct H0. subst.
+    destruct H5; try easy.
+    destruct H. destruct H. destruct H. destruct H. destruct H0. 
+    inversion H. subst. 
+    destruct H2; try easy. destruct H0. destruct H0. destruct H0. 
+    inversion H0. subst.
+    specialize(H2 m n G x1 x4 H3 H1). subst. easy.
+  }
+  subst. easy.
+  
+  inversion H. subst. inversion H0. subst.
+  specialize(IHG1 (S m) (S n) G Q1 Q0 H6 H5). subst. easy.
+Qed.
+
+Lemma wfL_after_incr : forall G1 m n,
+     wfL G1 -> wfL (incr_freeL m n G1).
+Proof.
+  induction G1 using local_ind_ref; intros; try easy.
+  - simpl in *.
+    constructor.
+  - revert m n H0 H. revert p.
+    induction lis; intros; try easy.
+    - inversion H. subst. clear H.
+      inversion H0. subst. inversion H5. subst.
+      specialize(SList_f a lis H2); intros.
+      destruct H.
+      - assert (wfL (incr_freeL m n (l_send p lis))).
+        {
+          apply IHlis; try easy.
+          inversion H0. subst. inversion H5. subst.
+          constructor; try easy.
+        }
+        destruct H6. subst.
+        - constructor. 
+          {
+            simpl. clear IHlis H3 H0 H4 H5 H2 H7 H1. 
+            revert m n p H. induction lis; intros; try easy.
+            specialize(SList_f a lis H); intros.
+            destruct H0.
+            - apply SList_b. apply IHlis; try easy.
+            - destruct H0. destruct H1. subst. 
+            simpl. destruct x; try easy.
+          }
+          constructor; try easy. left. easy.
+          {
+            clear IHlis H3 H0 H5 H2 H H1. clear p.
+            revert H4. revert m n. induction lis; intros; try easy. 
+            inversion H4. inversion H7. subst. clear H4 H7.
+            constructor. 
+            - destruct H1. subst. left. easy.
+            - destruct H. destruct H. destruct H. subst. right.
+              exists x. exists (incr_freeL m n x0). split; try easy. apply H0.
+              destruct H6; try easy. destruct H. destruct H. destruct H. inversion H. subst. easy.
+            - apply IHlis; try easy.
+          }
+        - destruct H6. destruct H6. destruct H6. subst. 
+          constructor; try easy.
+          {
+             apply SList_b.
+             clear IHlis H3 H0 H4 H5 H2 H8 H7 H1. clear x x0 p.
+             revert m n H.
+             induction lis; intros; try easy.
+             specialize(SList_f a lis H); intros.
+             destruct H0. apply SList_b. apply IHlis; try easy.
+             destruct H0. destruct H1. subst. destruct x. easy.
+          }
+          constructor. right. exists x. exists (incr_freeL m n x0).
+          split; try easy.
+          destruct H3; try easy. destruct H3. destruct H3. destruct H3. inversion H3. subst. 
+          apply H6; try easy.
+          {
+            clear IHlis H3 H0 H5 H2 H H1. clear p.
+            revert H4. revert m n. induction lis; intros; try easy. 
+            inversion H4. inversion H7. subst. clear H4 H7.
+            constructor. 
+            - destruct H1. subst. left. easy.
+            - destruct H. destruct H. destruct H. subst. right.
+              exists x1. exists (incr_freeL m n x2). split; try easy. apply H0.
+              destruct H6; try easy. destruct H. destruct H. destruct H. inversion H. subst. easy.
+            - apply IHlis; try easy.
+          }
+        - destruct H. destruct H1. subst.
+          destruct H6; try easy. destruct H. destruct H. destruct H. subst.
+          destruct H3; try easy. destruct H3. destruct H3. destruct H3. 
+          replace (Some x) with (Some (x2, x3)) in *. inversion H. subst. clear H H3 H4 H7 H5.
+          constructor; try easy. constructor; try easy.
+          right. exists x0. exists (incr_freeL m n x1).
+          split; try easy. apply H6; try easy.
+  - revert m n H0 H. revert p.
+    induction lis; intros; try easy.
+    - inversion H. subst. clear H.
+      inversion H0. subst. inversion H5. subst.
+      specialize(SList_f a lis H2); intros.
+      destruct H.
+      - assert (wfL (incr_freeL m n (l_recv p lis))).
+        {
+          apply IHlis; try easy.
+          inversion H0. subst. inversion H5. subst.
+          constructor; try easy.
+        }
+        destruct H6. subst.
+        - constructor. 
+          {
+            simpl. clear IHlis H3 H0 H4 H5 H2 H7 H1. 
+            revert m n p H. induction lis; intros; try easy.
+            specialize(SList_f a lis H); intros.
+            destruct H0.
+            - apply SList_b. apply IHlis; try easy.
+            - destruct H0. destruct H1. subst. 
+            simpl. destruct x; try easy.
+          }
+          constructor; try easy. left. easy.
+          {
+            clear IHlis H3 H0 H5 H2 H H1. clear p.
+            revert H4. revert m n. induction lis; intros; try easy. 
+            inversion H4. inversion H7. subst. clear H4 H7.
+            constructor. 
+            - destruct H1. subst. left. easy.
+            - destruct H. destruct H. destruct H. subst. right.
+              exists x. exists (incr_freeL m n x0). split; try easy. apply H0.
+              destruct H6; try easy. destruct H. destruct H. destruct H. inversion H. subst. easy.
+            - apply IHlis; try easy.
+          }
+        - destruct H6. destruct H6. destruct H6. subst. 
+          constructor; try easy.
+          {
+             apply SList_b.
+             clear IHlis H3 H0 H4 H5 H2 H8 H7 H1. clear x x0 p.
+             revert m n H.
+             induction lis; intros; try easy.
+             specialize(SList_f a lis H); intros.
+             destruct H0. apply SList_b. apply IHlis; try easy.
+             destruct H0. destruct H1. subst. destruct x. easy.
+          }
+          constructor. right. exists x. exists (incr_freeL m n x0).
+          split; try easy.
+          destruct H3; try easy. destruct H3. destruct H3. destruct H3. inversion H3. subst. 
+          apply H6; try easy.
+          {
+            clear IHlis H3 H0 H5 H2 H H1. clear p.
+            revert H4. revert m n. induction lis; intros; try easy. 
+            inversion H4. inversion H7. subst. clear H4 H7.
+            constructor. 
+            - destruct H1. subst. left. easy.
+            - destruct H. destruct H. destruct H. subst. right.
+              exists x1. exists (incr_freeL m n x2). split; try easy. apply H0.
+              destruct H6; try easy. destruct H. destruct H. destruct H. inversion H. subst. easy.
+            - apply IHlis; try easy.
+          }
+        - destruct H. destruct H1. subst.
+          destruct H6; try easy. destruct H. destruct H. destruct H. subst.
+          destruct H3; try easy. destruct H3. destruct H3. destruct H3. 
+          replace (Some x) with (Some (x2, x3)) in *. inversion H. subst. clear H H3 H4 H7 H5.
+          constructor; try easy. constructor; try easy.
+          right. exists x0. exists (incr_freeL m n x1).
+          split; try easy. apply H6; try easy.
+  - inversion H. subst.
+    constructor; try easy. apply IHG1; try easy.
+Qed.
+        
+  
+Lemma wfL_after_subst : forall Q G1 G2 m n,
+    wfL G1 -> wfL G2 -> subst_local m n G1 G2 Q -> wfL Q.
+Proof.
+  induction Q using local_ind_ref; intros; try easy.
+  - apply wfl_var.
+  - apply wfl_end.
+  - inversion H2; try easy. 
+    - subst.
+      apply wfL_after_incr. easy.
+    - subst.
+      inversion H1. subst.
+      revert H H0 H1 H2 H8 H5 H6.
+      revert p G1 m n xs.
+      induction lis; intros; try easy. 
+      - destruct xs; try easy.
+      - destruct xs; try easy.
+        specialize(SList_f o xs H5); intros. clear H5.
+        inversion H8. subst. clear H8. inversion H6. subst. clear H6.
+        destruct H3.
+        - constructor; try easy. apply SList_b.
+          {
+            clear IHlis H H0 H1 H2 H9 H7 H8. revert H11 H3. revert xs.
+            induction lis; intros; try easy.
+            destruct xs; try easy.
+            inversion H11. subst.
+            specialize(SList_f x l H3); intros. destruct H. 
+            - apply SList_b. apply IHlis with (xs := l); try easy.
+            - destruct H. destruct H0. subst. destruct lis; try easy.
+              destruct H2; try easy. destruct H. destruct H. destruct H. destruct H. destruct H0. subst. easy.
+          } 
+        - inversion H. subst. clear H.
+          assert (wfL (l_send p lis)). 
+          {
+            apply IHlis with (G1 := G1) (m := m) (n := n) (xs := xs); try easy.
+            inversion H1. subst. inversion H12. subst. clear H12.
+            constructor; try easy.
+            inversion H2. subst. inversion H13. subst. clear H13.
+            constructor; try easy.
+          }
+          inversion H. subst. constructor; try easy.
+          clear H11 H8 H10 H12 H13 IHlis.
+          destruct H6.
+          - left. easy.
+          - right. destruct H4. destruct H4. destruct H4. subst.
+            destruct H9; try easy. destruct H4. destruct H4. destruct H4. destruct H4. destruct H6. inversion H6. subst.
+            exists x1. exists x3. split; try easy.
+            destruct H7; try easy. destruct H4. destruct H4. destruct H4. inversion H4. subst. 
+            specialize(H5 G1 x0 m n). apply H5; try easy.
+        - destruct H3. destruct H4. subst.
+          destruct H9; try easy. destruct H3. destruct H3. destruct H3. destruct H3. destruct H4. inversion H3. subst.
+          destruct H7; try easy. destruct H4. destruct H4. destruct H4. inversion H4. subst. 
+          destruct lis; try easy.
+          constructor; try easy. constructor; try easy. right.
+          exists x. exists x2. split; try easy.
+          inversion H. subst. clear H. destruct H10; try easy. destruct H. destruct H. destruct H. inversion H. subst.
+          specialize(H7 G1 x3 m n). apply H7; try easy.
+  - inversion H2; try easy. 
+    - subst.
+      apply wfL_after_incr. easy.
+    - subst.
+      inversion H1. subst.
+      revert H H0 H1 H2 H8 H5 H6.
+      revert p G1 m n xs.
+      induction lis; intros; try easy. 
+      - destruct xs; try easy.
+      - destruct xs; try easy.
+        specialize(SList_f o xs H5); intros. clear H5.
+        inversion H8. subst. clear H8. inversion H6. subst. clear H6.
+        destruct H3.
+        - constructor; try easy. apply SList_b.
+          {
+            clear IHlis H H0 H1 H2 H9 H7 H8. revert H11 H3. revert xs.
+            induction lis; intros; try easy.
+            destruct xs; try easy.
+            inversion H11. subst.
+            specialize(SList_f x l H3); intros. destruct H. 
+            - apply SList_b. apply IHlis with (xs := l); try easy.
+            - destruct H. destruct H0. subst. destruct lis; try easy.
+              destruct H2; try easy. destruct H. destruct H. destruct H. destruct H. destruct H0. subst. easy.
+          } 
+        - inversion H. subst. clear H.
+          assert (wfL (l_recv p lis)). 
+          {
+            apply IHlis with (G1 := G1) (m := m) (n := n) (xs := xs); try easy.
+            inversion H1. subst. inversion H12. subst. clear H12.
+            constructor; try easy.
+            inversion H2. subst. inversion H13. subst. clear H13.
+            constructor; try easy.
+          }
+          inversion H. subst. constructor; try easy.
+          clear H11 H8 H10 H12 H13 IHlis.
+          destruct H6.
+          - left. easy.
+          - right. destruct H4. destruct H4. destruct H4. subst.
+            destruct H9; try easy. destruct H4. destruct H4. destruct H4. destruct H4. destruct H6. inversion H6. subst.
+            exists x1. exists x3. split; try easy.
+            destruct H7; try easy. destruct H4. destruct H4. destruct H4. inversion H4. subst. 
+            specialize(H5 G1 x0 m n). apply H5; try easy.
+        - destruct H3. destruct H4. subst.
+          destruct H9; try easy. destruct H3. destruct H3. destruct H3. destruct H3. destruct H4. inversion H3. subst.
+          destruct H7; try easy. destruct H4. destruct H4. destruct H4. inversion H4. subst. 
+          destruct lis; try easy.
+          constructor; try easy. constructor; try easy. right.
+          exists x. exists x2. split; try easy.
+          inversion H. subst. clear H. destruct H10; try easy. destruct H. destruct H. destruct H. inversion H. subst.
+          specialize(H7 G1 x3 m n). apply H7; try easy.
+  - inversion H1. subst.
+    apply wfL_after_incr; try easy.
+    subst.
+    specialize(IHQ G1 P (S m) (S n)). 
+    constructor. apply IHQ; try easy.
+    inversion H0. easy.
+Qed.
+  
+Lemma guard_break : forall x, (forall n, exists m, guardL n m (l_rec x)) -> exists T, multiS betaL (l_rec x) T /\  (forall n, exists m, guardL n m T) /\ (T = l_end \/ (exists p lis, T = l_send p lis \/ T = l_recv p lis)).
+Proof.
+  intros.
+  pose proof H as H1.
+  specialize(H1 1). destruct H1.
+  assert (exists T, multiS betaL (l_rec x) T /\
+  (T = l_end \/
+   (exists
+      (p : string) (lis : seq.seq (option (sort * local))),
+      T = l_send p lis \/ T = l_recv p lis))).
+  {
+    clear H. revert H0. revert x. induction x0; intros; try easy.
+    inversion H0. subst.
+    destruct Q; try easy.
+    - exists l_end.
+      split. apply multi_sing. constructor; try easy.
+      left. easy.
+    - exists (l_send s l).
+      split. apply multi_sing. constructor; try easy.
+      right. exists s. exists l. left. easy.
+    - exists (l_recv s l).
+      split. apply multi_sing. constructor; try easy.
+      right. exists s. exists l. right. easy.
+    - specialize(IHx0 Q H4). 
+      destruct IHx0. destruct H. exists x1. split; try easy.
+      apply multi_step with (y := (l_rec Q)).
+      constructor; try easy.
+      easy.
+  }
+  destruct H1. destruct H1. exists x1.
+  split; try easy. split; try easy.
+  clear H0 H2. clear x0.
+  revert H. induction H1; intros; try easy.
+  - inversion H. subst.
+    specialize(H0 n). destruct H0. 
+    inversion H0. subst.
+    - exists 0. apply gl_nil.
+    - subst. exists m.
+      specialize(subst_injL 0 0 (l_rec G) G y Q H3 H1); intros. subst. easy.
+  - inversion H. subst.
+    apply IHmultiS; try easy.
+    intros. specialize(H0 n0). destruct H0.
+    inversion H0. subst. exists 0. apply gl_nil.
+    subst. exists m.
+    specialize(subst_injL 0 0 (l_rec G) G y Q H4 H2); intros. subst. easy.
+Qed.
+
+
+
+
 End ltt.
 
 
