type/merge.v
@@ -1,0 +1,79 @@
+From SST Require Export type.global type.local type.isomorphism type.projection.
+Require Import List String Datatypes ZArith Relations PeanoNat.
+Open Scope list_scope.
+From Paco Require Import paco pacotac.
+Require Import Setoid Morphisms Coq.Program.Basics.
+Require Import Coq.Init.Datatypes.
+
+
+Lemma triv_merge : forall T T', isMerge T (Some T' :: nil) -> T = T'.
+Admitted.
+
+Lemma triv_merge2 : forall T xs, isMerge T xs -> isMerge T (None :: xs).
+Admitted. 
+
+Lemma triv_merge3 : forall T xs, isMerge T xs -> isMerge T (Some T :: xs).
+Admitted.
+
+Lemma merge_onth_recv : forall n p LQ ys1 gqT,
+      isMerge (ltt_recv p LQ) ys1 ->
+      onth n ys1 = Some gqT -> 
+      exists LQ', gqT = ltt_recv p LQ'.
+Admitted.
+
+Lemma merge_onth_send : forall n q LP ys0 gpT,
+      isMerge (ltt_send q LP) ys0 ->
+      onth n ys0 = Some gpT ->
+      exists LP', gpT = (ltt_send q LP').
+Admitted.
+
+Lemma merge_label_recv : forall Mp LQ' LQ0' T k l p,
+          isMerge (ltt_recv p LQ') Mp ->
+          onth k Mp = Some (ltt_recv p LQ0') ->
+          onth l LQ0' = Some T ->
+          exists T', onth l LQ' = Some T'.
+Admitted.
+
+Lemma merge_label_send : forall Mq LP' LP0' T k l q,
+          isMerge (ltt_send q LP') Mq ->
+          onth k Mq = Some (ltt_send q LP0') ->
+          onth l LP0' = Some T ->
+          exists T', onth l LP' = Some T'. 
+Admitted.
+
+Lemma merge_label_sendb : forall ys0 LP LP' ST n l q,
+      isMerge (ltt_send q LP) ys0 ->
+      onth n ys0 = Some (ltt_send q LP') ->
+      onth l LP = Some ST ->
+      onth l LP' = Some ST.
+Admitted.
+
+Lemma merge_same : forall ys ys0 ys1 p q l LP LQ S T S' T',
+      Forall
+        (fun u : option (sort * gtt) =>
+         u = None \/
+         (exists (s : sort) (g : gtt) (LP' LQ' : list (option (sort * ltt))) 
+          (T T' : sort * ltt),
+            u = Some (s, g) /\
+            projectionC g p (ltt_send q LP') /\
+            projectionC g q (ltt_recv p LQ') /\ onth l LP' = Some T /\ onth l LQ' = Some T')) ys ->
+      Forall2
+        (fun (u : option (sort * gtt)) (v : option ltt) =>
+         u = None /\ v = None \/
+         (exists (s : sort) (g : gtt) (t : ltt),
+            u = Some (s, g) /\ v = Some t /\ upaco3 projection bot3 g p t)) ys ys0 ->
+      isMerge (ltt_send q LP) ys0 ->
+      Forall2
+        (fun (u : option (sort * gtt)) (v : option ltt) =>
+         u = None /\ v = None \/
+         (exists (s : sort) (g : gtt) (t : ltt),
+            u = Some (s, g) /\ v = Some t /\ upaco3 projection bot3 g q t)) ys ys1 ->
+      isMerge (ltt_recv p LQ) ys1 ->
+      onth l LP = Some (S, T) ->
+      onth l LQ = Some (S', T') ->
+      Forall (fun u => u = None \/ (exists s g LP' LQ', u = Some (s, g) /\
+          projectionC g p (ltt_send q LP') /\ onth l LP' = Some (S, T) /\
+          projectionC g q (ltt_recv p LQ') /\ onth l LQ' = Some (S', T'))) ys.
+Proof.
+Admitted.
+ 
