type/proj_sub.v
@@ -1,0 +1,1103 @@
+From SST Require Export type.global type.local type.isomorphism type.projection type.merge.
+Require Import List String Datatypes ZArith Relations PeanoNat. 
+Open Scope list_scope.
+From Paco Require Import paco pacotac.
+Require Import Setoid Morphisms Coq.Program.Basics.
+Require Import Coq.Init.Datatypes.
+
+Lemma step_mon : monotone5 gttstep.
+Admitted.
+
+Lemma gttT_mon : monotone2 gttT.
+Admitted.
+
+Lemma in_some_implies_onth {A} : forall (x : A) xs,
+    In (Some x) xs -> exists n, onth n xs = Some x.
+Proof.
+  intros. revert H. revert x. 
+  induction xs; intros; try easy.
+  simpl in *. destruct H. exists 0. easy.
+  specialize(IHxs x H). destruct IHxs. exists (Nat.succ x0). easy.
+Qed.
+
+Lemma proj_inv_lis : forall Gl p q l s s' ys ctxG T T' SI LP LQ G',
+    (ishParts p Gl -> False) ->
+    (ishParts q Gl -> False) ->
+    Forall
+       (fun u : option gtt =>
+        u = None \/
+        (exists (g : gtt) (lsg : list (option (sort * gtt))),
+           u = Some g /\
+           g = gtt_send p q lsg /\
+           (exists (s' : sort) (Gjk : gtt) (Tp Tq : ltt),
+              onth l lsg = Some (s', Gjk) /\
+              projectionC Gjk p Tp /\ T = Tp /\ projectionC Gjk q Tq /\ T' = Tq) /\
+           Forall2
+             (fun (u0 : option (sort * gtt)) (v : option sort) =>
+              u0 = None /\ v = None \/
+              (exists (s : sort) (g' : gtt), u0 = Some (s, g') /\ v = Some s)) lsg SI))
+       ctxG ->
+    typ_gtth ctxG Gl (gtt_send s s' ys) ->
+    projectionC (gtt_send s s' ys) p (ltt_send q LP) -> 
+    projectionC (gtt_send s s' ys) q (ltt_recv p LQ) -> 
+    gttstepC (gtt_send s s' ys) G' p q l ->
+    (s = p /\ s' = q /\ exists Gk, onth l ys = Some Gk) \/
+    (s <> p /\ s' <> q /\ List.Forall (fun u => u = None \/ 
+        (exists s g LP' LQ' T T', u = Some(s, g) /\ projectionC g p (ltt_send q LP') /\ projectionC g q (ltt_recv p LQ') /\ 
+          onth l LP' = Some T /\ onth l LQ' = Some T')) ys).
+Proof.
+  intro Gl. induction Gl using gtth_ind_ref; intros; try easy.
+  - inversion H2. subst.
+    specialize(some_onth_implies_In n ctxG (gtt_send s s' ys) H8); intros.
+    specialize(Forall_forall (fun u : option gtt =>
+            u = None \/
+            (exists (g : gtt) (lsg : list (option (sort * gtt))),
+               u = Some g /\
+               g = gtt_send p q lsg /\
+               (exists (s' : sort) (Gjk : gtt) (Tp Tq : ltt),
+                  onth l lsg = Some (s', Gjk) /\
+                  projectionC Gjk p Tp /\
+                  T = Tp /\ projectionC Gjk q Tq /\ T' = Tq) /\
+               Forall2
+                 (fun (u0 : option (sort * gtt)) (v : option sort) =>
+                  u0 = None /\ v = None \/
+                  (exists (s : sort) (g' : gtt),
+                     u0 = Some (s, g') /\ v = Some s)) lsg SI)) ctxG); intros. destruct H7.
+    specialize(H7 H1). clear H1 H9. specialize(H7 (Some (gtt_send s s' ys)) H6).
+    destruct H7; try easy. destruct H1. destruct H1. destruct H1. destruct H7. destruct H9.
+    destruct H9. destruct H9. destruct H9. destruct H9. destruct H9. destruct H11. destruct H12. destruct H13. destruct H14. 
+    subst. inversion H1. subst.
+    left. split; try easy. split; try easy. exists (x1, x2). easy.
+  - inversion H3. subst. right. 
+    pinversion H4; try easy. subst.
+    assert False. apply H0. constructor. easy.
+    subst. split; try easy. 
+    pinversion H5; try easy. subst. split; try easy. 
+    rename p0 into p. rename q0 into q. 
+    pinversion H6; try easy. subst.
+    apply Forall_forall; intros; try easy. destruct x.
+    - right. destruct p0. clear H14 H16 H19.
+      specialize(in_some_implies_onth (s0, g) ys H7); intros. destruct H8. rename x into n.
+      assert(exists t t' g' g'', onth n ys1 = Some t /\ projectionC g q t /\ onth n ys0 = Some t' /\ projectionC g p t' /\ onth n xs = Some (s0, g') /\ typ_gtth ctxG g' g /\ onth n ys2 = Some (s0, g'') /\ gttstepC g g'' p q l /\ 
+              (forall (p q : string) (l : fin) (s0 s' : string)
+                 (ys : list (option (sort * gtt))) (ctxG : list (option gtt)) 
+                 (T T' : ltt) (SI : list (option sort)) (LP LQ : list (option (sort * ltt)))
+                 (G' : gtt),
+               (ishParts p g' -> False) ->
+               (ishParts q g' -> False) ->
+               Forall
+                 (fun u0 : option gtt =>
+                  u0 = None \/
+                  (exists (g0 : gtt) (lsg : list (option (sort * gtt))),
+                     u0 = Some g0 /\
+                     g0 = gtt_send p q lsg /\
+                     (exists (s'0 : sort) (Gjk : gtt) (Tp Tq : ltt),
+                        onth l lsg = Some (s'0, Gjk) /\
+                        projectionC Gjk p Tp /\ T = Tp /\ projectionC Gjk q Tq /\ T' = Tq) /\
+                     Forall2
+                       (fun (u1 : option (sort * gtt)) (v : option sort) =>
+                        u1 = None /\ v = None \/
+                        (exists (s1 : sort) (g' : gtt), u1 = Some (s1, g') /\ v = Some s1))
+                       lsg SI)) ctxG ->
+               typ_gtth ctxG g' (gtt_send s0 s' ys) ->
+               projectionC (gtt_send s0 s' ys) p (ltt_send q LP) ->
+               projectionC (gtt_send s0 s' ys) q (ltt_recv p LQ) ->
+               gttstepC (gtt_send s0 s' ys) G' p q l ->
+               s0 = p /\ s' = q /\ (exists Gk : sort * gtt, onth l ys = Some Gk) \/
+               s0 <> p /\
+               s' <> q /\
+               Forall
+                 (fun u0 : option (sort * gtt) =>
+                  u0 = None \/
+                  (exists
+                     (s1 : sort) (g0 : gtt) (LP' LQ' : list (option (sort * ltt))) 
+                   (T0 T'0 : sort * ltt),
+                     u0 = Some (s1, g0) /\
+                     projectionC g0 p (ltt_send q LP') /\
+                     projectionC g0 q (ltt_recv p LQ') /\
+                     onth l LP' = Some T0 /\ onth l LQ' = Some T'0)) ys)
+      ).
+      {
+        clear H7 H28 H27 H26 H25 H21 H20 H24 H13 H12 H11 H6 H5 H4 H3 H1 H0 H10.
+        clear H23 H18.
+        clear H2. revert H8 H34 H33 H15 H17 H22 H. revert xs p q l s s' ctxG T T' SI LP LQ ys2 ys0 ys1 s0 g n.
+        induction ys; intros; try easy. destruct n; try easy. 
+        destruct ys2; try easy. destruct ys1; try easy. destruct xs; try easy. destruct ys0; try easy.
+        inversion H34. subst. clear H34. inversion H. subst. clear H.
+        inversion H33. subst. clear H33. inversion H22. subst. clear H22.
+        inversion H17. subst. clear H17. inversion H15. subst. clear H15.
+        
+        destruct n.
+        - simpl in *. subst.
+          destruct H3; try easy. destruct H. destruct H. destruct H. destruct H. destruct H0.
+          inversion H. subst. clear H.
+          clear H16 H13 H11 H6 H4 H5 IHys.
+          destruct H1; try easy. destruct H. destruct H. destruct H. destruct H0. 
+          inversion H. subst. clear H.
+          destruct H9; try easy. destruct H. destruct H. destruct H. destruct H. destruct H4. 
+          inversion H. subst. clear H.
+          destruct H10; try easy. destruct H. destruct H. destruct H. destruct H. destruct H4.
+          inversion H. subst. clear H.
+          destruct H12; try easy. destruct H. destruct H. destruct H. destruct H. destruct H4.
+          inversion H4. subst. clear H4.
+          destruct H2; try easy. destruct H. destruct H. destruct H. inversion H. subst.
+          exists x4. exists x5. exists x3. exists x1. pclearbot. easy.
+        - simpl in *.
+          apply IHys; try easy.
+      }
+      clear H34 H33 H22 H17 H15 H. clear H11 H12 H13.
+      destruct H9. destruct H. destruct H. destruct H. destruct H. destruct H9. destruct H11.
+      destruct H12. destruct H13. destruct H14. destruct H15. destruct H16.
+      rename x0 into gpT. rename x1 into g'. rename x2 into g''. rename x into gqT.
+      destruct g; try easy. pinversion H16; try easy. apply step_mon.
+      specialize(H17 p q l s1 s2 l0 ctxG T T' SI).
+      specialize(merge_onth_send n q LP ys0 gpT H18 H11); intros. destruct H19. subst.
+      specialize(merge_onth_recv n p LQ ys1 gqT H23 H); intros. destruct H19. subst.
+      rename x0 into LQ'. rename x into LP'.
+      specialize(H17 LP' LQ' g''). 
+      exists s0. exists (gtt_send s1 s2 l0). exists LP'. exists LQ'.
+      assert (ishParts p g' -> False).
+      {
+        intros. apply H0.
+        - case_eq (eqb p s); intros.
+          assert (p = s). apply eqb_eq; try easy. subst. apply ha_sendp.
+        - case_eq (eqb p s'); intros.
+          assert (p = s'). apply eqb_eq; try easy. subst. apply ha_sendq.
+        - assert (p <> s). apply eqb_neq; try easy. 
+          assert (p <> s'). apply eqb_neq; try easy.
+          apply ha_sendr with (n := n) (s := s0) (g := g'); try easy. 
+      }
+      assert (ishParts q g' -> False).
+      {
+        intros. apply H1.
+        - case_eq (eqb q s); intros.
+          assert (q = s). apply eqb_eq; try easy. subst. apply ha_sendp.
+        - case_eq (eqb q s'); intros.
+          assert (q = s'). apply eqb_eq; try easy. subst. apply ha_sendq.
+        - assert (q <> s). apply eqb_neq; try easy. 
+          assert (q <> s'). apply eqb_neq; try easy.
+          apply ha_sendr with (n := n) (s := s0) (g := g'); try easy.
+      }
+      assert (s1 = p /\ s2 = q /\ (exists Gk : sort * gtt, onth l l0 = Some Gk) \/
+      s1 <> p /\
+      s2 <> q /\
+      Forall
+        (fun u0 : option (sort * gtt) =>
+         u0 = None \/
+         (exists (s1 : sort) (g0 : gtt) (LP' LQ' : list (option (sort * ltt))) 
+          (T0 T'0 : sort * ltt),
+            u0 = Some (s1, g0) /\
+            projectionC g0 p (ltt_send q LP') /\
+            projectionC g0 q (ltt_recv p LQ') /\ onth l LP' = Some T0 /\ onth l LQ' = Some T'0)) l0).
+      {
+        apply H17; try easy.
+      }
+      
+      destruct H29.
+      - destruct H29. destruct H30. destruct H31. subst. clear H17 H2.
+        pinversion H9; try easy. subst. pinversion H12; try easy. subst.
+        destruct x.
+        assert(exists T0 T'0, onth l LP' = Some T0 /\ onth l LQ' = Some T'0).
+        {
+          clear H0 H1 H3 H4 H5 H6 H10 H19 H24 H20 H21 H22 H25 H26 H27 H28 H7.
+          clear H8 H9 H12 H11 H13 H14 H15 H16 H18 H23 H30 H H29 H35 H32.
+          clear xs s s' ys ctxG T T' s0 LP LQ ys2 ys0 ys1 s0 g' g''. clear SI n.
+          revert H31 H34 H37.
+          revert p q l LQ' LP' s1 g. induction l0; intros; try easy.
+          destruct l; try easy.
+          destruct LQ'; try easy. destruct LP'; try easy. 
+          inversion H34. subst. inversion H37. subst. clear H34 H37.
+          destruct l. simpl in *. subst.
+          destruct H2; try easy. destruct H. destruct H. destruct H. destruct H. destruct H0.
+          inversion H. subst. clear H.
+          destruct H3; try easy. destruct H. destruct H. destruct H. destruct H. destruct H0.
+          inversion H. subst. clear H.
+          exists (x2, x4). exists (x2, x1). split; try easy.
+          specialize(IHl0 p q l LQ' LP' s1 g). apply IHl0; try easy.
+        }
+        destruct H2. destruct H2. exists x. exists x0.
+        split. easy. split. pfold. easy. split. pfold. easy. easy.
+        apply proj_mon. apply proj_mon. 
+      - destruct H29. destruct H30. 
+        inversion H14. subst.
+        - clear H31 H17 H18 H23 H16 H15 H13 H14 H11 H12 H H9 H8 H7 H28 H27 H26 H25 H22 H21 H20 H24 H19.
+          clear H10 H6 H5 H4 H3 H1 H0.
+          assert False.
+          clear LQ' LP' g'' n s0 ys0 ys1 ys2. clear LP LQ ys s s'. clear xs.
+          revert H32 H30 H29 H2. revert p q l T T' SI s1 s2 l0 n0.
+          induction ctxG; intros; try easy. destruct n0; try easy.
+          inversion H2. subst. clear H2. 
+          destruct n0. simpl in H32.
+          - subst. destruct H1; try easy. destruct H. destruct H. destruct H.
+            destruct H0. inversion H. subst. inversion H4. subst. easy.
+          - specialize(IHctxG p q l T T' SI s1 s2 l0 n0). apply IHctxG; try easy.
+            easy.
+        - subst.
+          assert (exists k s4 g2 LP' LQ' T0 T'0, onth k l0 = Some(s4, g2) /\ projectionC g2 p (ltt_send q LP') /\ projectionC g2 q (ltt_recv p LQ') /\ onth l LP' = Some T0 /\ onth l LQ' = Some T'0).
+          {
+            clear H30 H29 H17 H18 H23 H16 H15 H13 H14 H11 H12 H9 H8 H7 H28 H27 H26 H25 H22 H21 H.
+            clear H20 H24 H19 H10 H6 H5 H4 H3 H2 H1 H0. revert H38 H36 H31.
+            revert xs p q l s s' ys ctxG T T' SI LP LQ ys2 ys0 ys1 s0 s1 s2 l0 n g'' LQ' LP'.
+            induction xs0; try easy.
+            intros.
+            destruct l0; try easy. inversion H38. subst. inversion H31. subst. clear H31 H38.
+            specialize(SList_f a xs0 H36); intros. destruct H.
+            assert (exists (k : fin) (s4 : sort) (g2 : gtt) (LP' LQ'0 : list (option (sort * ltt))) 
+        (T0 T'0 : sort * ltt),
+          onth k l0 = Some (s4, g2) /\
+          projectionC g2 p (ltt_send q LP') /\
+          projectionC g2 q (ltt_recv p LQ'0) /\ onth l LP' = Some T0 /\ onth l LQ'0 = Some T'0).
+            {
+              apply IHxs0 with (p := p) (q := q) (l0 := l0) (ctxG := ctxG); try easy.
+            }
+            destruct H0. exists (Nat.succ x). easy.
+            
+            destruct H. destruct H0. subst. destruct l0; try easy.
+            destruct H2; try easy. destruct H. destruct H. destruct H. destruct H. destruct H0.
+            inversion H. subst.
+            destruct H1; try easy. destruct H0. destruct H0. destruct H0. destruct H0. destruct H0.
+            destruct H0. destruct H0. destruct H1. destruct H5. destruct H6. inversion H0. subst.
+            exists 0. exists x. exists x3. exists x4. exists x5. exists x6. exists x7. easy.
+          }
+          destruct H32. destruct H32. destruct H32. destruct H32. destruct H32. 
+          destruct H32. destruct H32. destruct H32. destruct H33. destruct H34. 
+          destruct H35. rename x2 into LP0'. rename x3 into LQ0'. clear H31.
+          
+          pinversion H9; try easy. subst.
+          pinversion H12; try easy. subst. 
+          clear H38 H36 H30 H29 H17 H18 H23 H16 H15 H13 H14 H11 H8 H7 H28 H27.
+          clear H26 H25 H22 H21 H20 H24 H19 H10 H6 H5 H4 H3 H2 H1 H0 H.
+          assert (exists t t', onth x ys3 = Some t /\ projectionC x1 q t /\ onth x ys4 = Some t' /\ projectionC x1 p t').
+          {
+              clear H48 H45 H44 H43 H42 H41 H34 H33 H47 H52 H12 H9 .
+              clear xs s s' ys T T' SI LP LQ ys2 ys0 ys1. clear xs0 g''. clear n. clear ctxG.
+              revert H32 H35 H37 H46 H51. 
+              revert p q l s0 s1 s2 LQ' LP' x x0 x1 LP0' LQ0' x4 x5 ys3 ys4.
+              induction l0; intros; try easy.
+              - destruct x; try easy.
+              - destruct ys3; try easy. destruct ys4; try easy.
+              inversion H46. subst. inversion H51. subst. clear H46 H51.
+              destruct x.
+              - simpl in H32. subst. destruct H2; try easy. destruct H. destruct H. destruct H.
+                destruct H. destruct H0. inversion H. subst.
+                destruct H3; try easy. destruct H0. destruct H0. destruct H0. destruct H0. destruct H2.
+                inversion H0. subst.
+                exists x3. exists x6. pclearbot. easy.
+              - simpl. apply IHl0 with (l := l) (x0 := x0) (x4 := x4) (x5 := x5) (LP0' := LP0') (LQ0' := LQ0'); try easy.
+          }
+          destruct H. destruct H. destruct H. destruct H0. destruct H1.
+          specialize(proj_inj H2 H33); intros. subst.
+          specialize(proj_inj H0 H34); intros. subst.
+          rename ys3 into Mp. rename ys4 into Mq. rename x into k.
+          specialize(merge_label_send Mq LP' LP0' x4 k l q H52 H1 H35); intros.
+          destruct H3. 
+          specialize(merge_label_recv Mp LQ' LQ0' x5 k l p H47 H H37); intros.
+          destruct H4.
+          exists x. exists x2. pclearbot. split. easy. split. pfold. easy. split. pfold. easy. easy.
+        apply proj_mon.
+        apply proj_mon.
+    - left. easy.
+    apply step_mon. apply proj_mon. apply proj_mon.
+Qed.
+
+Lemma _3_19_1_helper : forall p q l G G' LP LQ S T S' T',
+  wfgC G -> 
+  projectionC G p (ltt_send q LP) ->
+  onth l LP = Some(S, T) ->
+  projectionC G q (ltt_recv p LQ) -> 
+  onth l LQ = Some(S', T') ->
+  gttstepC G G' p q l -> 
+  projectionC G' p T.
+Proof.
+  intros.
+  specialize(_a_29_s G p q LP LQ S T S' T' l H H0 H1 H2 H3); intros.
+  destruct H5. rename x into Gl. clear H.
+  revert H0 H1 H2 H3 H4 H5. revert p q l G G' LP LQ S S' T T'.
+  induction Gl using gtth_ind_ref; intros.
+  - destruct H5. destruct H. destruct H. destruct H. destruct H5. destruct H6. destruct H7. destruct H8. destruct H9.
+    rename x1 into Sn. rename x0 into SI. rename x into ctxG. 
+    inversion H. subst.
+    specialize(some_onth_implies_In n ctxG G H13); intros.
+    specialize(Forall_forall (fun u : option gtt =>
+        u = None \/
+        (exists (g : gtt) (lsg : list (option (sort * gtt))),
+           u = Some g /\
+           g = gtt_send p q lsg /\
+           (exists (s' : sort) (Gjk : gtt) (Tp Tq : ltt),
+              onth l lsg = Some (s', Gjk) /\
+              projectionC Gjk p Tp /\ T = Tp /\ projectionC Gjk q Tq /\ T' = Tq) /\
+           Forall2
+             (fun (u0 : option (sort * gtt)) (v : option sort) =>
+              u0 = None /\ v = None \/ (exists (s : sort) (g' : gtt), u0 = Some (s, g') /\ v = Some s))
+             lsg SI)) ctxG); intros. destruct H12.
+    specialize(H12 H7). clear H7 H14. 
+    specialize(H12 (Some G) H11). destruct H12; try easy.
+    destruct H7. destruct H7. destruct H7. destruct H12. destruct H14.
+    destruct H14. destruct H14. destruct H14. destruct H14. destruct H14. destruct H16. destruct H17. destruct H18.
+    subst. inversion H7. subst. clear H7.
+    pinversion H4; try easy. subst. specialize(eq_trans H25 H14); intros. inversion H7. subst. easy.
+    apply step_mon.
+  - rename p into s. rename q into s'. rename p0 into p. rename q0 into q.
+    destruct H5. destruct H5. destruct H5. destruct H5. destruct H6. destruct H7. destruct H8. destruct H9. destruct H10.
+    rename x into ctxG. rename x1 into Sn. rename x0 into SI. 
+    inversion H5. subst. 
+    pinversion H0; try easy. subst.
+    assert False. apply H6. constructor. easy.
+    pinversion H2; try easy. subst.
+    pinversion H4; try easy. subst. 
+    
+    specialize(proj_inv_lis (gtth_send s s' xs) p q l s s' ys ctxG T T' SI LP LQ (gtt_send s s' ys2)); intros.
+    assert (s = p /\ s' = q /\ (exists Gk : sort * gtt, onth l ys = Some Gk) \/
+      s <> p /\
+      s' <> q /\
+      Forall
+        (fun u : option (sort * gtt) =>
+         u = None \/
+         (exists (s : sort) (g : gtt) (LP' LQ' : list (option (sort * ltt))) 
+          (T T' : sort * ltt),
+            u = Some (s, g) /\
+            projectionC g p (ltt_send q LP') /\
+            projectionC g q (ltt_recv p LQ') /\ onth l LP' = Some T /\ onth l LQ' = Some T')) ys).
+    {
+      pclearbot.
+      apply H12; try easy. pfold. easy. pfold. easy. pfold. easy.
+    }
+    destruct H13; try easy. destruct H13. destruct H14.
+    clear H15 H16 H19 H27 H28 H29 H20 H13 H14 H12.
+        
+    assert (List.Forall (fun u => u = None \/ (exists s g, u = Some (s, g) /\ projectionC g p T)) ys2).
+    {
+      clear H5 H4 H2 H0 H17.
+      specialize(merge_same ys ys0 ys1 p q l LP LQ S T S' T' H34 H22 H23 H32 H33 H1 H3); intros.
+      clear H34 H33 H22.
+      clear H23 H30 H21 H24 H25 H26 H31 H32 H38 H3 H1. 
+      revert H0 H39 H18 H8 H7 H6 H H9 H10 H11. clear ys0 ys1 LP LQ. 
+      revert s s' p q l S S' T T' ys ys2 ctxG SI Sn.
+      induction xs; intros; try easy.
+      - destruct ys; try easy. destruct ys2; try easy.
+      - destruct ys; try easy. destruct ys2; try easy.
+        inversion H0. subst. clear H0. inversion H39. subst. clear H39.
+        inversion H18. subst. clear H18. inversion H. subst. clear H.
+        specialize(IHxs s s' p q l S S' T T' ys ys2 ctxG SI Sn).
+        assert (Forall
+         (fun u : option (sort * gtt) =>
+          u = None \/ (exists (s : sort) (g : gtt), u = Some (s, g) /\ projectionC g p T)) ys2).
+        {
+          apply IHxs; try easy.
+          - intros. apply H7.
+            - case_eq (eqb q s); intros.
+              assert (q = s). apply eqb_eq; try easy. subst. apply ha_sendp.
+            - case_eq (eqb q s'); intros.
+              assert (q = s'). apply eqb_eq; try easy. subst. apply ha_sendq.
+            - assert (q <> s). apply eqb_neq; try easy. 
+              assert (q <> s'). apply eqb_neq; try easy.
+              inversion H; try easy. subst.
+              apply ha_sendr with (n := Nat.succ n) (s := s0) (g := g); try easy.
+          - intros. apply H6.
+            - case_eq (eqb p s); intros.
+              assert (p = s). apply eqb_eq; try easy. subst. apply ha_sendp.
+            - case_eq (eqb p s'); intros.
+              assert (p = s'). apply eqb_eq; try easy. subst. apply ha_sendq.
+            - assert (p <> s). apply eqb_neq; try easy. 
+              assert (p <> s'). apply eqb_neq; try easy.
+              inversion H; try easy. subst.
+              apply ha_sendr with (n := Nat.succ n) (s := s0) (g := g); try easy.
+        }
+        clear H14 H15 H13 H4 IHxs.
+        constructor; try easy.
+        destruct H5. destruct H0. left. easy.
+        destruct H0. destruct H0. destruct H0. destruct H0. destruct H1. subst. right.
+        exists x. exists x1. split; try easy.
+        destruct H12; try easy. destruct H0. destruct H0. destruct H0. destruct H0. destruct H1.
+        inversion H1. subst. clear H1.
+        destruct H3; try easy. destruct H0. destruct H0. destruct H0. destruct H0. destruct H0.
+        destruct H1. destruct H3. destruct H12. inversion H0. subst. clear H0.
+        destruct H2; try easy. destruct H0. destruct H0. destruct H0.
+        inversion H0. subst.
+        rename x4 into Gl. rename x0 into G. rename x1 into G'. rename x6 into LQ. rename x5 into LP.
+        specialize(H2 p q l G G' LP LQ S S' T T').
+        apply H2; try easy. destruct H4; try easy.
+        exists ctxG. exists SI. exists Sn. split. easy.
+        clear H2 H H4.
+        - split. intros. apply H6. 
+          - case_eq (eqb p s); intros.
+            assert (p = s). apply eqb_eq; try easy. subst. apply ha_sendp.
+          - case_eq (eqb p s'); intros.
+            assert (p = s'). apply eqb_eq; try easy. subst. apply ha_sendq.
+          - assert (p <> s). apply eqb_neq; try easy. 
+            assert (p <> s'). apply eqb_neq; try easy.
+            apply ha_sendr with (n := 0) (s := x2) (g := Gl); try easy.
+        - split; try easy. intros. apply H7.
+          - case_eq (eqb q s); intros.
+            assert (q = s). apply eqb_eq; try easy. subst. apply ha_sendp.
+          - case_eq (eqb q s'); intros.
+            assert (q = s'). apply eqb_eq; try easy. subst. apply ha_sendq.
+          - assert (q <> s). apply eqb_neq; try easy. 
+            assert (q <> s'). apply eqb_neq; try easy.
+            apply ha_sendr with (n := 0) (s := x2) (g := Gl); try easy.
+    }
+    
+    assert(exists ys3, Forall2 (fun u v => (u = None /\ v = None) \/ (exists s g t, u = Some(s, g) /\ v = Some t /\ projectionC g p t)) ys2 ys3 /\ isMerge T ys3).
+    {
+      clear H34 H38 H31 H30 H26 H25 H24 H21 H33 H32 H23 H22 H11 H10 H9 H8 H7 H6 H5 H4 H3 H2 H1 H0 H.
+      revert H17 H18 H12 H39.
+      revert s s' xs p q l LP LQ S S' T T' ys ctxG SI Sn ys0 ys1.
+      induction ys2; intros; try easy.
+      - destruct ys; try easy. destruct xs; try easy.
+      - destruct ys; try easy. destruct xs; try easy.
+        inversion H18. subst. inversion H12. subst. inversion H39. subst. clear H18 H12 H39.
+        specialize(SList_f o0 xs H17); intros.
+        destruct H.
+        - assert (exists ys3, Forall2
+            (fun (u : option (sort * gtt)) (v : option ltt) =>
+             (u = None /\ v = None) \/
+             (exists (s : sort) (g : gtt) (t : ltt), u = Some (s, g) /\ v = Some t /\ projectionC g p t))
+            ys2 ys3 /\ isMerge T ys3).
+          {
+            apply IHys2 with (xs := xs) (q := q) (l := l) (ys := ys) (ctxG := ctxG); try easy.
+          }
+          destruct H0. clear IHys2.
+          - destruct H6. destruct H5. subst. 
+            exists (None :: x). split. constructor; try easy. left. easy.
+            destruct H0.
+            apply triv_merge2; try easy.
+          - destruct H5. destruct H5. destruct H5. destruct H5. destruct H6. subst.
+            destruct H2; try easy. destruct H2. destruct H2. destruct H2. destruct H2. destruct H5.
+            inversion H5. subst. 
+            destruct H1; try easy. destruct H1. destruct H1. destruct H1. inversion H1. subst.
+            exists (Some T :: x). split.
+            constructor; try easy. right. exists x0. exists x1. exists T. easy.
+            apply triv_merge3; try easy.
+          - destruct H. destruct H0. subst.
+            destruct ys; try easy. destruct ys2; try easy. clear H3 H8 H4 IHys2.
+            destruct H2; try easy. destruct H. destruct H. destruct H. destruct H. destruct H0.
+            inversion H. subst.
+            destruct H6; try easy. destruct H0. destruct H0. destruct H0. destruct H0. destruct H3.
+            inversion H0. subst.
+            destruct H1; try easy. destruct H1. destruct H1. destruct H1. inversion H1. subst.
+            exists (Some T :: nil). split.
+            constructor; try easy. right. exists x0. exists x2. exists T. easy.
+            unfold isMerge. easy.
+    }
+    destruct H13. destruct H13. pfold.
+    apply proj_cont with (ys := x); try easy.
+    clear H H0 H1 H2 H3 H4 H5 H6 H7 H8 H9 H10 H11 H17 H18 H22 H23 H32 H33 H21 H24 H25 H26 H30 H31 H38 H39 H34 H12 H14.
+    clear s s' xs q l LP LQ S S' T T' ys ctxG SI Sn ys0 ys1.
+    revert H13. revert p x.
+    induction ys2; intros; try easy.
+    - destruct x; try easy.
+    - destruct x; try easy.
+      inversion H13. subst. clear H13.
+      specialize(IHys2 p x H4). constructor; try easy. clear IHys2 H4.
+      destruct H2. left. easy. 
+      destruct H. destruct H. destruct H. destruct H. destruct H0. subst.
+      right. exists x0. exists x1. exists x2. split. easy. split. easy. left. easy.
+    apply step_mon.
+    apply proj_mon.
+    apply proj_mon.
+Qed.
+
+Lemma _3_19_2_helper : forall p q l G G' LP LQ S T S' T',
+  wfgC G -> 
+  projectionC G p (ltt_send q LP) ->
+  onth l LP = Some(S, T) ->
+  projectionC G q (ltt_recv p LQ) -> 
+  onth l LQ = Some(S', T') ->
+  gttstepC G G' p q l -> 
+  projectionC G' q T'.
+Proof.
+  intros.
+  specialize(_a_29_s G p q LP LQ S T S' T' l H H0 H1 H2 H3); intros.
+  destruct H5. rename x into Gl. clear H.
+  revert H0 H1 H2 H3 H4 H5. revert p q l G G' LP LQ S S' T T'.
+  induction Gl using gtth_ind_ref; intros.
+  - destruct H5. destruct H. destruct H. destruct H. destruct H5. destruct H6. destruct H7. destruct H8. destruct H9.
+    rename x1 into Sn. rename x0 into SI. rename x into ctxG. 
+    inversion H. subst.
+    specialize(some_onth_implies_In n ctxG G H13); intros.
+    specialize(Forall_forall (fun u : option gtt =>
+        u = None \/
+        (exists (g : gtt) (lsg : list (option (sort * gtt))),
+           u = Some g /\
+           g = gtt_send p q lsg /\
+           (exists (s' : sort) (Gjk : gtt) (Tp Tq : ltt),
+              onth l lsg = Some (s', Gjk) /\
+              projectionC Gjk p Tp /\ T = Tp /\ projectionC Gjk q Tq /\ T' = Tq) /\
+           Forall2
+             (fun (u0 : option (sort * gtt)) (v : option sort) =>
+              u0 = None /\ v = None \/ (exists (s : sort) (g' : gtt), u0 = Some (s, g') /\ v = Some s))
+             lsg SI)) ctxG); intros. destruct H12.
+    specialize(H12 H7). clear H7 H14. 
+    specialize(H12 (Some G) H11). destruct H12; try easy.
+    destruct H7. destruct H7. destruct H7. destruct H12. destruct H14.
+    destruct H14. destruct H14. destruct H14. destruct H14. destruct H14. destruct H16. destruct H17. destruct H18.
+    subst. inversion H7. subst. clear H7.
+    pinversion H4; try easy. subst. specialize(eq_trans H25 H14); intros. inversion H7. subst. easy.
+    apply step_mon.
+  - rename p into s. rename q into s'. rename p0 into p. rename q0 into q.
+    destruct H5. destruct H5. destruct H5. destruct H5. destruct H6. destruct H7. destruct H8. destruct H9. destruct H10.
+    rename x into ctxG. rename x1 into Sn. rename x0 into SI. 
+    inversion H5. subst. 
+    pinversion H0; try easy. subst.
+    assert False. apply H6. constructor. easy.
+    pinversion H2; try easy. subst.
+    pinversion H4; try easy. subst. 
+    
+    specialize(proj_inv_lis (gtth_send s s' xs) p q l s s' ys ctxG T T' SI LP LQ (gtt_send s s' ys2)); intros.
+    assert (s = p /\ s' = q /\ (exists Gk : sort * gtt, onth l ys = Some Gk) \/
+      s <> p /\
+      s' <> q /\
+      Forall
+        (fun u : option (sort * gtt) =>
+         u = None \/
+         (exists (s : sort) (g : gtt) (LP' LQ' : list (option (sort * ltt))) 
+          (T T' : sort * ltt),
+            u = Some (s, g) /\
+            projectionC g p (ltt_send q LP') /\
+            projectionC g q (ltt_recv p LQ') /\ onth l LP' = Some T /\ onth l LQ' = Some T')) ys).
+    {
+      pclearbot.
+      apply H12; try easy. pfold. easy. pfold. easy. pfold. easy.
+    }
+    destruct H13; try easy. destruct H13. destruct H14.
+    clear H15 H16 H19 H27 H28 H29 H20 H13 H14 H12.
+        
+    assert (List.Forall (fun u => u = None \/ (exists s g, u = Some (s, g) /\ projectionC g q T')) ys2).
+    {
+      clear H5 H4 H2 H0 H17.
+      specialize(merge_same ys ys0 ys1 p q l LP LQ S T S' T' H34 H22 H23 H32 H33 H1 H3); intros.
+      clear H34 H33 H22.
+      clear H23 H30 H21 H24 H25 H26 H31 H32 H38 H3 H1. 
+      revert H0 H39 H18 H8 H7 H6 H H9 H10 H11. clear ys0 ys1 LP LQ. 
+      revert s s' p q l S S' T T' ys ys2 ctxG SI Sn.
+      induction xs; intros; try easy.
+      - destruct ys; try easy. destruct ys2; try easy.
+      - destruct ys; try easy. destruct ys2; try easy.
+        inversion H0. subst. clear H0. inversion H39. subst. clear H39.
+        inversion H18. subst. clear H18. inversion H. subst. clear H.
+        specialize(IHxs s s' p q l S S' T T' ys ys2 ctxG SI Sn).
+        assert (Forall
+         (fun u : option (sort * gtt) =>
+          u = None \/ (exists (s : sort) (g : gtt), u = Some (s, g) /\ projectionC g q T')) ys2).
+        {
+          apply IHxs; try easy.
+          - intros. apply H7.
+            - case_eq (eqb q s); intros.
+              assert (q = s). apply eqb_eq; try easy. subst. apply ha_sendp.
+            - case_eq (eqb q s'); intros.
+              assert (q = s'). apply eqb_eq; try easy. subst. apply ha_sendq.
+            - assert (q <> s). apply eqb_neq; try easy. 
+              assert (q <> s'). apply eqb_neq; try easy.
+              inversion H; try easy. subst.
+              apply ha_sendr with (n := Nat.succ n) (s := s0) (g := g); try easy.
+          - intros. apply H6.
+            - case_eq (eqb p s); intros.
+              assert (p = s). apply eqb_eq; try easy. subst. apply ha_sendp.
+            - case_eq (eqb p s'); intros.
+              assert (p = s'). apply eqb_eq; try easy. subst. apply ha_sendq.
+            - assert (p <> s). apply eqb_neq; try easy. 
+              assert (p <> s'). apply eqb_neq; try easy.
+              inversion H; try easy. subst.
+              apply ha_sendr with (n := Nat.succ n) (s := s0) (g := g); try easy.
+        }
+        clear H14 H15 H13 H4 IHxs.
+        constructor; try easy.
+        destruct H5. destruct H0. left. easy.
+        destruct H0. destruct H0. destruct H0. destruct H0. destruct H1. subst. right.
+        exists x. exists x1. split; try easy.
+        destruct H12; try easy. destruct H0. destruct H0. destruct H0. destruct H0. destruct H1.
+        inversion H1. subst. clear H1.
+        destruct H3; try easy. destruct H0. destruct H0. destruct H0. destruct H0. destruct H0.
+        destruct H1. destruct H3. destruct H12. inversion H0. subst. clear H0.
+        destruct H2; try easy. destruct H0. destruct H0. destruct H0.
+        inversion H0. subst.
+        rename x4 into Gl. rename x0 into G. rename x1 into G'. rename x6 into LQ. rename x5 into LP.
+        specialize(H2 p q l G G' LP LQ S S' T T').
+        apply H2; try easy. destruct H4; try easy.
+        exists ctxG. exists SI. exists Sn. split. easy.
+        clear H2 H H4.
+        - split. intros. apply H6. 
+          - case_eq (eqb p s); intros.
+            assert (p = s). apply eqb_eq; try easy. subst. apply ha_sendp.
+          - case_eq (eqb p s'); intros.
+            assert (p = s'). apply eqb_eq; try easy. subst. apply ha_sendq.
+          - assert (p <> s). apply eqb_neq; try easy. 
+            assert (p <> s'). apply eqb_neq; try easy.
+            apply ha_sendr with (n := 0) (s := x2) (g := Gl); try easy.
+        - split; try easy. intros. apply H7.
+          - case_eq (eqb q s); intros.
+            assert (q = s). apply eqb_eq; try easy. subst. apply ha_sendp.
+          - case_eq (eqb q s'); intros.
+            assert (q = s'). apply eqb_eq; try easy. subst. apply ha_sendq.
+          - assert (q <> s). apply eqb_neq; try easy. 
+            assert (q <> s'). apply eqb_neq; try easy.
+            apply ha_sendr with (n := 0) (s := x2) (g := Gl); try easy.
+    }
+    
+    assert(exists ys3, Forall2 (fun u v => (u = None /\ v = None) \/ (exists s g t, u = Some(s, g) /\ v = Some t /\ projectionC g q t)) ys2 ys3 /\ isMerge T' ys3).
+    {
+      clear H34 H38 H31 H30 H26 H25 H24 H21 H33 H32 H23 H22 H11 H10 H9 H8 H7 H6 H5 H4 H3 H2 H1 H0 H.
+      revert H17 H18 H12 H39.
+      revert s s' xs p q l LP LQ S S' T T' ys ctxG SI Sn ys0 ys1.
+      induction ys2; intros; try easy.
+      - destruct ys; try easy. destruct xs; try easy.
+      - destruct ys; try easy. destruct xs; try easy.
+        inversion H18. subst. inversion H12. subst. inversion H39. subst. clear H18 H12 H39.
+        specialize(SList_f o0 xs H17); intros.
+        destruct H.
+        - assert (exists ys3, Forall2
+            (fun (u : option (sort * gtt)) (v : option ltt) =>
+             (u = None /\ v = None) \/
+             (exists (s : sort) (g : gtt) (t : ltt), u = Some (s, g) /\ v = Some t /\ projectionC g q t))
+            ys2 ys3 /\ isMerge T' ys3).
+          {
+            apply IHys2 with (xs := xs) (p := p) (l := l) (ys := ys) (ctxG := ctxG); try easy.
+          }
+          destruct H0. clear IHys2.
+          - destruct H6. destruct H5. subst. 
+            exists (None :: x). split. constructor; try easy. left. easy.
+            destruct H0.
+            apply triv_merge2; try easy.
+          - destruct H5. destruct H5. destruct H5. destruct H5. destruct H6. subst.
+            destruct H2; try easy. destruct H2. destruct H2. destruct H2. destruct H2. destruct H5.
+            inversion H5. subst. 
+            destruct H1; try easy. destruct H1. destruct H1. destruct H1. inversion H1. subst.
+            exists (Some T' :: x). split.
+            constructor; try easy. right. exists x0. exists x1. exists T'. easy.
+            apply triv_merge3; try easy.
+          - destruct H. destruct H0. subst.
+            destruct ys; try easy. destruct ys2; try easy. clear H3 H8 H4 IHys2.
+            destruct H2; try easy. destruct H. destruct H. destruct H. destruct H. destruct H0.
+            inversion H. subst.
+            destruct H6; try easy. destruct H0. destruct H0. destruct H0. destruct H0. destruct H3.
+            inversion H0. subst.
+            destruct H1; try easy. destruct H1. destruct H1. destruct H1. inversion H1. subst.
+            exists (Some T' :: nil). split.
+            constructor; try easy. right. exists x0. exists x2. exists T'. easy.
+            unfold isMerge. easy.
+    }
+    destruct H13. destruct H13. pfold.
+    apply proj_cont with (ys := x); try easy.
+    clear H H0 H1 H2 H3 H4 H5 H6 H7 H8 H9 H10 H11 H17 H18 H22 H23 H32 H33 H21 H24 H25 H26 H30 H31 H38 H39 H34 H12 H14.
+    clear s s' xs p l LP LQ S S' T T' ys ctxG SI Sn ys0 ys1.
+    revert H13. revert q x.
+    induction ys2; intros; try easy.
+    - destruct x; try easy.
+    - destruct x; try easy.
+      inversion H13. subst. clear H13.
+      specialize(IHys2 q x H4). constructor; try easy. clear IHys2 H4.
+      destruct H2. left. easy. 
+      destruct H. destruct H. destruct H. destruct H. destruct H0. subst.
+      right. exists x0. exists x1. exists x2. split. easy. split. easy. left. easy.
+    apply step_mon.
+    apply proj_mon.
+    apply proj_mon.
+Qed.
+
+Lemma SList_to_In {A} : forall (xs : list (option A)),
+    SList xs ->
+    exists t, In (Some t) xs.
+Proof.
+  induction xs; intros; try easy.
+  specialize(SList_f a xs H); intros.
+  destruct H0.
+  specialize(IHxs H0). destruct IHxs. exists x. right. easy.
+  destruct H0. destruct H1. subst. exists x. left. easy.
+Qed.
+
+Lemma projection_step_label : forall G G' p q l LP LQ,
+  wfgC G ->
+  projectionC G p (ltt_send q LP) ->
+  projectionC G q (ltt_recv p LQ) ->
+  gttstepC G G' p q l ->
+  exists LS LS' LT LT', onth l LP = Some(LS, LT) /\ onth l LQ = Some(LS', LT').
+Proof.
+  intros.
+  specialize(_a_29_11 G p q LP H H0); intros.
+  destruct H3. rename x into Gl.
+  assert (exists ctxJ : list (option gtt),
+       typ_gtth ctxJ Gl G /\
+       (ishParts p Gl -> False) /\
+       Forall
+         (fun u : option gtt =>
+          u = None \/
+          (exists (g : gtt) (lsg : list (option (sort * gtt))),
+             u = Some g /\
+             g = gtt_send p q lsg)) ctxJ). 
+  {
+    destruct H3. exists x. destruct H3. destruct H4. split. easy. split. easy.
+    clear H4 H3 H2 H1 H0 H. clear Gl LQ l. clear G G'.
+    revert H5. revert LP p q. induction x; intros; try easy.
+    inversion H5. subst. clear H5. specialize(IHx LP p q H2). constructor; try easy. clear H2 IHx.
+    destruct H1. left. easy.
+    destruct H. destruct H. destruct H. destruct H0. right. exists x0. exists x1. easy.
+  } 
+  clear H3. rename H4 into H3.
+  revert H0 H1 H2 H3. clear H.
+  revert G G' p q l LP LQ.
+  induction Gl using gtth_ind_ref; intros; try easy.
+  - destruct H3. destruct H. destruct H3. inversion H. subst. 
+    specialize(some_onth_implies_In n x G H7); intros.
+    specialize(Forall_forall (fun u : option gtt =>
+        u = None \/
+        (exists (g : gtt) (lsg : list (option (sort * gtt))),
+           u = Some g /\
+           g = gtt_send p q lsg)) x); intros.
+    destruct H6. specialize(H6 H4). clear H8. specialize(H6 (Some G) H5). clear H5 H4.
+    destruct H6; try easy. destruct H4. destruct H4. destruct H4. inversion H4.
+    subst.
+    pinversion H1; try easy. subst.
+    pinversion H2; try easy. subst.
+    pinversion H0; try easy. subst.
+    clear H9 H16 H15 H14 H11 H8 H10 H7 H3 H0 H1 H2 H4 H H17. clear n x.
+    revert H12 H18 H20. revert G' p q LP LQ x1 s.
+    induction l; intros; try easy.
+    - destruct x1; try easy.
+      destruct LP; try easy. destruct LQ; try easy.
+      inversion H20. subst. clear H20. inversion H12. subst. clear H12. 
+      simpl in *. subst.
+      destruct H2; try easy. destruct H. destruct H. destruct H. destruct H. destruct H0.
+      inversion H. subst.
+      destruct H3; try easy. destruct H0. destruct H0. destruct H0. destruct H0. destruct H2.
+      inversion H0. subst.
+      exists x3. exists x3. exists x2. exists x5. easy.
+    - destruct x1; try easy. destruct LP; try easy. destruct LQ; try easy.
+      inversion H12. subst. inversion H20. subst.
+      specialize(IHl G' p q LP LQ x1 s). apply IHl; try easy.
+    apply proj_mon.
+    apply step_mon. 
+    apply proj_mon.
+  - destruct H3. destruct H3. destruct H4. 
+    rename p into s. rename q into s0. rename p0 into p. rename q0 into q.
+    specialize(_a_29_part x (gtth_send s s0 xs) G p q LP LQ H3 H0 H1 H4); intros.
+    inversion H3. subst.
+    pinversion H1. subst.
+    - assert False. apply H4. constructor. easy.
+    pinversion H0; try easy. subst. 
+    specialize(SList_to_In xs H12); intros. destruct H7.
+    specialize(Forall_forall (fun u : option (sort * gtth) =>
+       u = None \/
+       (exists (s : sort) (g : gtth),
+          u = Some (s, g) /\
+          (forall (G G' : gtt) (p q : string) (l : fin) (LP LQ : list (option (sort * ltt))),
+           projectionC G p (ltt_send q LP) ->
+           projectionC G q (ltt_recv p LQ) ->
+           gttstepC G G' p q l ->
+           (exists ctxJ : list (option gtt),
+              typ_gtth ctxJ g G /\
+              (ishParts p g -> False) /\
+              Forall
+                (fun u0 : option gtt =>
+                 u0 = None \/
+                 (exists (g0 : gtt) (lsg : list (option (sort * gtt))),
+                    u0 = Some g0 /\
+                    g0 = gtt_send p q lsg)) ctxJ) ->
+           exists (LS LS' : sort) (LT LT' : ltt),
+             onth l LP = Some (LS, LT) /\ onth l LQ = Some (LS', LT')))) xs); intros.
+    destruct H8. specialize(H8 H). clear H H9.
+    specialize(H8 (Some x0) H7). destruct H8; try easy. destruct H. destruct H.
+    destruct H. inversion H. subst. clear H. rename x2 into G.
+    specialize(in_some_implies_onth (x1, G) xs H7); intros. destruct H. clear H7. rename x0 into n.
+    rename x into ctxG.
+    pinversion H2; try easy. subst.
+    assert(exists g g' t t', onth n ys = Some(x1, g) /\ typ_gtth ctxG G g /\ onth n ys0 = Some t /\ projectionC g q t /\
+           onth n ys1 = Some t' /\ projectionC g p t' /\ onth n ys2 = Some (x1, g') /\ gttstepC g g' p q l).
+    {
+      clear H2 H1 H0 H3 H4 H5 H6 H12 H10 H11 H14 H18 H22 H23 H24 H28 H8 H16 H19 H20 H21 H25 H26 H29 H34.
+      clear LP LQ. clear s s0.
+      revert H H27 H17 H13. revert H35. 
+      revert xs p q ys ctxG ys0 ys1 x1 G. revert l ys2.
+      induction n; intros; try easy.
+      - destruct xs; try easy.
+        destruct ys; try easy. destruct ys0; try easy. destruct ys1; try easy.
+        inversion H27. subst. inversion H13. subst. inversion H17. subst. inversion H35. subst. clear H27 H13 H17 H35.
+        simpl in *. subst.
+        destruct H4; try easy. destruct H. destruct H. destruct H. destruct H. destruct H0. 
+        inversion H. subst. clear H. 
+        destruct H3; try easy. destruct H. destruct H. destruct H. destruct H. destruct H0.
+        inversion H. subst. clear H.
+        destruct H6; try easy. destruct H. destruct H. destruct H. destruct H. destruct H0.
+        inversion H. subst. clear H.
+        destruct H2; try easy. destruct H. destruct H. destruct H. destruct H. destruct H0.
+        inversion H. subst. clear H.
+        exists x3. exists x6. exists x5. exists x4. pclearbot. destruct H2; try easy.
+      - destruct xs; try easy. destruct ys; try easy. destruct ys0; try easy. destruct ys1; try easy.
+        inversion H27. subst. inversion H17. subst. inversion H13. subst. inversion H35. subst. apply IHn with (xs := xs); try easy.
+    }
+    destruct H7. destruct H7. destruct H7. destruct H7. destruct H7. destruct H9. destruct H15. destruct H30.
+    destruct H31. destruct H32. destruct H33. 
+    rename x into G0'. rename x2 into LP0. rename x3 into LQ0. rename x0 into G''.
+    specialize(H8 G0' G'' p q l).
+    specialize(merge_onth_recv n p LQ ys0 LP0 H18 H15); intros. destruct H37 as [LQ' H37].
+    specialize(merge_onth_send n q LP ys1 LQ0 H28 H31); intros. destruct H38 as [LP' H38].
+    subst.
+    specialize(H8 LP' LQ' H32 H30 H36).
+    assert (exists (LS LS' : sort) (LT LT' : ltt), onth l LP' = Some (LS, LT) /\ onth l LQ' = Some (LS', LT')).
+    {
+      apply H8; try easy.
+      exists ctxG. split. easy. split; try easy.
+      intros. apply H4.
+      - case_eq (eqb p s); intros.
+        assert (p = s). apply eqb_eq; try easy. subst. apply ha_sendp.
+      - case_eq (eqb p s0); intros.
+        assert (p = s0). apply eqb_eq; try easy. subst. apply ha_sendq.
+      - assert (p <> s). apply eqb_neq; try easy. 
+        assert (p <> s0). apply eqb_neq; try easy.
+        apply ha_sendr with (n := n) (s := x1) (g := G); try easy.
+    }
+    destruct H37. destruct H37. destruct H37. destruct H37. destruct H37. 
+    
+    specialize(merge_label_send ys1 LP LP' (x, x2) n l q H28 H31 H37); intros.
+    destruct H39. 
+    specialize(merge_label_recv ys0 LQ LQ' (x0, x3) n l p H18 H15 H38); intros.
+    destruct H40. destruct x4. destruct x5.
+    exists s1. exists s2. exists l0. exists l1. easy.
+  apply step_mon.
+  apply proj_mon.
+  apply proj_mon.
+Qed.
+
+Lemma projection_step_label_s : forall G p q l LP LQ ST,
+  wfgC G ->
+  projectionC G p (ltt_send q LP) ->
+  onth l LP = Some ST -> 
+  projectionC G q (ltt_recv p LQ) ->
+  exists LS' LT', onth l LQ = Some(LS', LT').
+Proof.
+  intros.
+  specialize(_a_29_11 G p q LP H H0); intros.
+  destruct H3. rename x into Gl.
+  assert (exists ctxJ : list (option gtt),
+       typ_gtth ctxJ Gl G /\
+       (ishParts p Gl -> False) /\
+       Forall
+         (fun u : option gtt =>
+          u = None \/
+          (exists (g : gtt) (lsg : list (option (sort * gtt))),
+             u = Some g /\
+             g = gtt_send p q lsg)) ctxJ). 
+  {
+    destruct H3. exists x. destruct H3. destruct H4. split. easy. split. easy.
+    clear H4 H3 H2 H1 H0 H. clear Gl LQ l. clear G.
+    revert H5. revert LP p q. induction x; intros; try easy.
+    inversion H5. subst. clear H5. specialize(IHx LP p q H2). constructor; try easy. clear H2 IHx.
+    destruct H1. left. easy.
+    destruct H. destruct H. destruct H. destruct H0. right. exists x0. exists x1. easy.
+  }
+  clear H3. clear H.
+  revert H4 H2 H1 H0. revert G p q l LP LQ ST.
+  induction Gl using gtth_ind_ref; intros.
+  - destruct H4. destruct H. destruct H3.
+    inversion H. subst. 
+    specialize(some_onth_implies_In n x G H7); intros.
+    specialize(Forall_forall (fun u : option gtt =>
+        u = None \/
+        (exists (g : gtt) (lsg : list (option (sort * gtt))),
+           u = Some g /\
+           g = gtt_send p q lsg)) x); intros.
+    destruct H6. specialize(H6 H4 (Some G) H5). clear H4 H8.
+    destruct H6; try easy. destruct H4. destruct H4. destruct H4. inversion H4. subst.
+    pinversion H0; try easy. subst.
+    pinversion H2; try easy. subst.
+    clear H10 H14 H9 H11 H0 H7 H5 H2 H3 H H4. clear n x.
+    revert H16 H13 H1. revert p q LP LQ ST x1.
+    induction l; intros.
+    - destruct LP; try easy. destruct x1; try easy. destruct LQ; try easy.
+      inversion H16. inversion H13. subst. clear H16 H13.
+      simpl in H1. subst.
+      destruct H9; try easy. destruct H. destruct H. destruct H. destruct H. destruct H0.
+      inversion H0. subst.
+      destruct H3; try easy. destruct H. destruct H. destruct H. destruct H. destruct H2.
+      inversion H. subst. 
+      exists x3. exists x5. easy.
+    - destruct LP; try easy. destruct x1; try easy. destruct LQ; try easy.
+      inversion H16. inversion H13. subst.
+      specialize(IHl p q LP LQ ST x1). apply IHl; try easy.
+    apply proj_mon. 
+    apply proj_mon.
+  - destruct H4. destruct H3. destruct H4. 
+    inversion H3. subst.
+    specialize(SList_to_In xs H11); intros. destruct H6.
+    specialize(in_some_implies_onth x0 xs H6); intros. destruct H7. rename x1 into n.
+    specialize(Forall_forall (fun u : option (sort * gtth) =>
+       u = None \/
+       (exists (s : sort) (g : gtth),
+          u = Some (s, g) /\
+          (forall (G : gtt) (p q : string) (l : fin) (LP LQ : list (option (sort * ltt)))
+             (ST : sort * ltt),
+           (exists ctxJ : list (option gtt),
+              typ_gtth ctxJ g G /\
+              (ishParts p g -> False) /\
+              Forall
+                (fun u0 : option gtt =>
+                 u0 = None \/
+                 (exists (g0 : gtt) (lsg : list (option (sort * gtt))),
+                    u0 = Some g0 /\ g0 = gtt_send p q lsg)) ctxJ) ->
+           projectionC G q (ltt_recv p LQ) ->
+           onth l LP = Some ST ->
+           projectionC G p (ltt_send q LP) ->
+           exists (LS' : sort) (LT' : ltt), onth l LQ = Some (LS', LT')))) xs); intros.
+    destruct H8. specialize(H8 H (Some x0) H6). clear H9 H. destruct H8; try easy.
+    destruct H. destruct H. destruct H. inversion H. subst.
+    pinversion H0. subst.
+    assert False. apply H4. constructor. easy.
+    subst.
+    pinversion H2; try easy. subst.
+    rename p into s. rename q into s'. rename p0 into p. rename q0 into q.
+    rename x1 into s0. rename x2 into g. rename x into ctxG.
+    clear H H6 H11 H2 H0 H3.
+    assert(exists g' t t', onth n ys = Some (s0, g') /\ typ_gtth ctxG g g' /\ onth n ys0 = Some t /\ projectionC g' p t 
+          /\ onth n ys1 = Some t' /\ projectionC g' q t').
+    {
+      clear H25 H21 H18 H17 H20 H16 H15 H14 H5 H1 H4 H8. clear ST LP LQ. clear s s'. clear l.
+      revert H24 H19 H12 H7. revert xs p q ctxG ys s0 g ys0 ys1.
+      induction n; intros.
+      - destruct xs; try easy. destruct ys; try easy. destruct ys0; try easy. destruct ys1; try easy.
+        inversion H24. inversion H19. inversion H12. subst. clear H24 H19 H12.
+        simpl in H7. subst.
+        destruct H16; try easy. destruct H. destruct H. destruct H. destruct H. destruct H0.
+        inversion H. subst. clear H.
+        destruct H9; try easy. destruct H. destruct H. destruct H. destruct H. destruct H0.
+        inversion H. subst. clear H.
+        destruct H2; try easy. destruct H. destruct H. destruct H. destruct H. destruct H0. 
+        inversion H. subst. clear H.
+        simpl. exists x1. exists x4. exists x5. pclearbot. easy.
+      - destruct xs; try easy. destruct ys; try easy. destruct ys0; try easy. destruct ys1; try easy.
+        inversion H24. inversion H19. inversion H12. subst. clear H24 H19 H12.
+        specialize(IHn xs p q ctxG ys s0 g ys0 ys1). apply IHn; try easy.
+    }
+    destruct H. destruct H. destruct H. destruct H. destruct H0. destruct H2. destruct H3. destruct H6.
+    clear H24 H19 H12.
+    rename x into g'. 
+    specialize(merge_onth_recv n p LQ ys1 x1 H25 H6); intros. destruct H10. subst.
+    specialize(merge_onth_send n q LP ys0 x0 H20 H2); intros. destruct H10. subst.
+    rename x1 into LP'. rename x into LQ'.
+    
+    specialize(H8 g' p q l LP' LQ' ST).
+    specialize(merge_label_sendb ys0 LP LP' ST n l q H20 H2 H1); intros. 
+    assert (exists (LS' : sort) (LT' : ltt), onth l LQ' = Some (LS', LT')).
+    {
+      apply H8; try easy.
+      exists ctxG. split; try easy. split; try easy.
+      intros. apply H4. apply ha_sendr with (n := n) (s := s0) (g := g); try easy.
+      
+    }
+    destruct H11. destruct H11.
+    specialize(merge_label_recv ys1 LQ LQ' (x, x0) n l p H25 H6 H11); intros. destruct H12.
+    destruct x1. exists s1. exists l0. easy.
+  apply proj_mon.
+  apply proj_mon.
+Qed.
+
+Lemma _3_19_1 : forall p q l G G' LP LQ S T S' T' xs,
+  wfgC G ->
+  projectionC G p (ltt_send q LP) ->
+  subtypeC (ltt_send q (extendLis l (Datatypes.Some (S, T)))) (ltt_send q LP) ->
+  projectionC G q (ltt_recv p LQ) ->
+  onth l xs = Some (S', T') ->
+  subtypeC (ltt_recv p xs) (ltt_recv p LQ) ->
+  gttstepC G G' p q l ->
+  exists L, 
+  projectionC G' p L /\ subtypeC T L. 
+Proof.
+  intros.
+  specialize(_3_19_1_helper p q l G G' LP LQ); intros.
+  specialize(subtype_send_inv q (extendLis l (Some (S, T))) LP H1); intros.
+  specialize(subtype_recv_inv p xs LQ H4); intros.
+  specialize(projection_step_label G G' p q l LP LQ H H0 H2 H5); intros.
+  destruct H9. destruct H9. destruct H9. destruct H9. destruct H9.
+  rename x into s. rename x0 into s'. rename x1 into t. rename x2 into t'.
+  
+  specialize(H6 s t s' t' H H0 H9 H2 H10 H5).
+  exists t. split; try easy.
+  
+  clear H10 H8 H6 H5 H4 H3 H2 H1 H0 H. clear s' t' xs T' S' LQ G G' p q.
+  revert H9 H7. revert LP S T t s.
+  induction l; intros; try easy.
+  - destruct LP; try easy. inversion H7. subst.
+    destruct H2; try easy. destruct H. destruct H. destruct H. destruct H. destruct H. destruct H0.
+    destruct H1. inversion H. subst. simpl in H9. inversion H9. subst. easy.
+  - destruct LP; try easy. inversion H7. subst. specialize(IHl LP S T t s). apply IHl; try easy.
+Qed.
+
+
+Lemma _3_19_2 : forall p q l G G' LP LQ S T S' T' xs,
+  wfgC G ->
+  projectionC G p (ltt_send q LP) ->
+  subtypeC (ltt_send q (extendLis l (Datatypes.Some (S, T)))) (ltt_send q LP) ->
+  projectionC G q (ltt_recv p LQ) ->
+  onth l xs = Some (S', T') ->
+  subtypeC (ltt_recv p xs) (ltt_recv p LQ) ->
+  gttstepC G G' p q l ->
+  exists L, 
+  projectionC G' q L /\ subtypeC T' L. 
+Proof.
+  intros.
+  specialize(_3_19_2_helper p q l G G' LP LQ); intros.
+  specialize(subtype_send_inv q (extendLis l (Some (S, T))) LP H1); intros.
+  specialize(subtype_recv_inv p xs LQ H4); intros.
+  specialize(projection_step_label G G' p q l LP LQ H H0 H2 H5); intros.
+  destruct H9. destruct H9. destruct H9. destruct H9. destruct H9.
+  rename x into s. rename x0 into s'. rename x1 into t. rename x2 into t'.
+  
+  specialize(H6 s t s' t' H H0 H9 H2 H10 H5).
+  exists t'. split; try easy.
+  
+  clear H9 H7 H6 H5 H4 H2 H1 H0 H.
+  clear s t S T LP G G' p q.
+  revert H3 H8 H10. revert LQ S' T' xs t' s'.
+  induction l; intros.
+  - destruct LQ; try easy. destruct xs; try easy.
+    inversion H8. subst. simpl in *. subst.
+    destruct H2; try easy. destruct H. destruct H. destruct H. destruct H. destruct H. destruct H0.
+    destruct H1. inversion H0. inversion H. subst. easy.
+  - destruct LQ; try easy. destruct xs; try easy. 
+    inversion H8. subst. simpl in *. 
+    specialize(IHl LQ S' T' xs t' s'). apply IHl; try easy.
+Qed.
+  
+Lemma _3_19_3_helper : forall G G' p q s l L1 L2 S T S' T',
+      wfgC G ->
+      projectionC G p (ltt_send q L1) ->
+      onth l L1 = Some (S, T) ->
+      projectionC G q (ltt_recv p L2) ->
+      onth l L2 = Some (S', T') ->
+      gttstepC G G' p q l ->
+      s <> q ->
+      s <> p ->
+      projectionC G s T -> 
+      exists T', (T = T' /\ T = ltt_end) \/ 
+                 (exists r xs, p <> r /\ q <> r /\ T = T' /\ T = ltt_send r xs) \/ 
+                 (exists r xs ys, p <> r /\ q <> r /\ T = ltt_recv r xs /\ T' = ltt_recv r ys /\ Forall2R (fun u v => u = None \/ u = v) ys xs /\ (SList xs -> SList ys)).
+Proof.
+Admitted.
+
+Lemma _3_19_step : forall p q l G L1 L2 S T S' T',
+  wfgC G ->
+  projectionC G p (ltt_send q L1) -> 
+  onth l L1 = Some(S, T) ->
+  projectionC G q (ltt_recv p L2) -> 
+  onth l L2 = Some(S', T') ->
+  exists G', gttstepC G G' p q l.
+Proof.
+  intros.
+  
+Admitted.
+
+
+Lemma _3_19_h : forall p q l G L1 L2 S T xs y,
+  wfgC G ->
+  projectionC G p (ltt_send q L1) -> 
+  subtypeC (ltt_send q (extendLis l (Datatypes.Some(S,T)))) (ltt_send q L1) ->
+  projectionC G q (ltt_recv p L2) -> 
+  onth l xs = Some y ->
+  subtypeC (ltt_recv p xs) (ltt_recv p L2) -> 
+  exists G', gttstepC G G' p q l.
+Proof.
+  intros. 
+  
+Admitted.
+
+
+
+
